fix + refactor

NS/Misc.v
@@ -5,9 +5,7 @@ Require Import Coq.Strings.String.
 Require Import Coq.Arith.PeanoNat.
 Require Import Coq.Arith.EqNat.
 Require Import Coq.Bool.Bool.
-Require Import Coq.Logic.FunctionalExtensionality.
 Require Import Coq.Logic.Eqdep.
-Require Import Coq.Program.Equality.
 
 Notation "a <| b" := (a b) (at level 102, right associativity, only parsing).
 Notation "a << b" := (fun x => a (b x)) (at level 101, right associativity, only parsing).
@@ -112,68 +110,73 @@ match a, b with
 | _, _ => None
 end.
 
-Inductive Option_Forall {A: Type}: (A -> Prop) -> option A -> Prop :=
-| Option_Forall_None: forall (P: A -> Prop), Option_Forall P None
-| Option_Forall_Some: forall (P: A -> Prop) (a: A), P a -> Option_Forall P (Some a).
+Inductive Option_Forall {A: Type} (P: A -> Prop): option A -> Prop :=
+| Option_Forall_None: Option_Forall P None
+| Option_Forall_Some: forall a, P a -> Option_Forall P (Some a).
 
-Definition js_record (A: Set): Set := list (string * A).
+Ltac remove_existTs :=
+  repeat lazymatch goal with
+  | H : existT (fun x0 : Set => x0) ?T ?a = existT (fun x1 : Set => x1) ?T ?b |- _ => apply inj_pair2 in H
+  end.
+Ltac clear_obvious :=
+  repeat lazymatch goal with
+  | H : ?T = ?T |- _ => clear H
+  | H : True |- _ => clear H
+  end.
+Ltac inv H := inversion H; remove_existTs; clear_obvious; subst; clear H; try discriminate.
+Ltac if_some tac H := lazymatch H with | None => idtac | @None => idtac | Some ?H => tac H | ?H => idtac H; fail "must be None or Some" end.
 
-Fixpoint js_record_has_key {A: Set} (key: string) (a: js_record A): bool :=
-match a with
-| nil => false
-| cons (x_key, _) xs => String.eqb key x_key || js_record_has_key key xs
-end.
+Local Ltac invert_eqs' n :=
+  match n with
+  | 0 => idtac "warning: invert_eqs' gave up"
+  | S ?n =>
+      lazymatch goal with
+      | H : ?f ?a ?a0 ?a1 ?a2 ?a3 ?a4 ?a5 = ?f ?b ?b0 ?b1 ?b2 ?b3 ?b4 ?b5 |- _ => inv H; invert_eqs' n
+      | H : ?f ?a ?a0 ?a1 ?a2 ?a3 ?a4 = ?f ?b ?b0 ?b1 ?b2 ?b3 ?b4 |- _ => inv H; invert_eqs' n
+      | H : ?f ?a ?a0 ?a1 ?a2 ?a3 = ?f ?b ?b0 ?b1 ?b2 ?b3 |- _ => inv H; invert_eqs' n
+      | H : ?f ?a ?a0 ?a1 ?a2 = ?f ?b ?b0 ?b1 ?b2 |- _ => inv H; invert_eqs' n
+      | H : ?f ?a ?a0 ?a1 = ?f ?b ?b0 ?b1 |- _ => inv H; invert_eqs' n
+      | H : ?f ?a ?a0 = ?f ?b ?b0 |- _ => inv H; invert_eqs' n
+      | H : ?f ?a = ?f ?b |- _ => inv H; invert_eqs' n
+      | H : ?a = nil |- _ => rewrite H in *; clear H; invert_eqs' n
+      end
+  end.
+Ltac invert_eqs := invert_eqs' 33.
 
-Fixpoint js_record_assoc {A: Set} (key: string) (a: js_record A): option A :=
-match a with
-| nil => None
-| cons (x_key, x) xs => if String.eqb key x_key then Some x else js_record_assoc key xs
-end.
+Ltac revert_with t :=
+  repeat lazymatch goal with
+  | H : context[t] |- _ => revert H
+  end.
 
-Definition map_js_record {A B: Set} (f: A -> B) (a: js_record A): js_record B :=
-  List.map (fun x => match x with (name, value) => (name, f value) end) a.
+Ltac assert_specialize H :=
+  let tH := type of H in
+  match tH with
+  | ?tHH -> ?tHC =>
+      let HH := fresh "HH" in
+      assert (HH : tHH); [clear H | specialize (H HH); clear HH]
+  | ?tHH <-> ?tHC => apply proj1 in H; assert_specialize H
+  end.
 
-Fixpoint js_record_fields_superset {A B: Set} (a: js_record A) (b: js_record B): bool :=
-match b with
-| nil => true
-| cons (b_key, _) bs => js_record_has_key b_key a && js_record_fields_superset a bs
-end.
+Ltac split_with H :=
+  split; [destruct H as [H _] | destruct H as [_ H]].
 
-Definition js_record_fields_eqb {A B: Set} (a: js_record A) (b: js_record B): bool :=
-  js_record_fields_superset a b && js_record_fields_superset b a.
+Ltac left_right_with H :=
+  destruct H as [H | H]; [left | right].
 
-Fixpoint js_record_zip_with {A B C: Set} (f: A -> B -> C) (a: js_record A) (b: js_record B): js_record C :=
-match a with
-| nil => nil
-| cons (x_key, x) xs =>
-    cons_opt (option_map ((fun z => (x_key, z)) << f x) (js_record_assoc x_key b)) (js_record_zip_with f xs b)
-end.
+Ltac destruct_var H := is_var H; destruct H.
 
-Definition JsRecordForall {A: Set} (P: A -> Prop) : js_record A -> Prop := List.Forall (P << snd).
-
-Definition JsRecordHasKey {A: Set} (key: string): js_record A -> Prop :=
-  List.Exists (fun '(key', _) => key = key').
-
-Definition JsRecordSuperKeys {A: Set} (xs ys: js_record A): Prop :=
-  forall k, JsRecordHasKey k xs -> JsRecordHasKey k ys.
-
-Definition JsRecordEqKeys {A: Set} (xs ys: js_record A): Prop :=
-  forall k, JsRecordHasKey k xs <-> JsRecordHasKey k ys.
-
-Inductive JsRecordEqKeys0 {A: Set}: js_record A -> js_record A -> Prop :=
-| JsRecordEqKeys0_nil : JsRecordEqKeys0 nil nil
-| JsRecordEqKeys0_add : forall (k: string) (vx vy: A) (xs ys xs' ys': js_record A), JsRecordEqKeys0 xs ys -> List.Add (k, vx) xs xs' -> List.Add (k, vy) ys ys' -> JsRecordEqKeys0 xs' ys'
-.
-
-Inductive JsRecordAdd {A: Set} (kx: string) (vx: A) : js_record A -> js_record A -> Prop :=
-| JsRecordAdd_head : forall (xs: js_record A), JsRecordAdd kx vx xs ((kx, vx) :: xs)%list
-| JsRecordAdd_cons : forall (kx0: string) (vx0: A) (xs xs': js_record A), kx0 <> kx -> JsRecordAdd kx vx xs xs' -> JsRecordAdd kx vx ((kx0, vx0) :: xs)%list ((kx0, vx0) :: xs')%list
-.
-
-Inductive JsRecordNoDup {A: Set} : js_record A -> Prop :=
-| JsRecordNoDup_nil : JsRecordNoDup nil
-| JsRecordNoDup_cons : forall kx vx xs, JsRecordNoDup xs -> not (JsRecordHasKey kx xs) -> JsRecordNoDup ((kx, vx) :: xs)%list
-.
+Ltac destruct' H :=
+  destruct_var H || lazymatch H with
+  | ?P => is_ind P || is_constructor P || is_const P
+  | ?P ?H0 => is_ind P; destruct' H0
+  | ?P ?H0 ?H1 => is_ind P; destruct' H0; destruct' H1
+  | ?P ?H0 ?H1 ?H2 => is_ind P; destruct' H0; destruct' H1; destruct' H2
+  | ?P ?H0 ?H1 ?H2 ?H3 => is_ind P; destruct' H0; destruct' H1; destruct' H2; destruct' H3
+  | ?P ?H0 ?H1 ?H2 ?H3 ?H4 => is_ind P; destruct' H0; destruct' H1; destruct' H2; destruct' H3; destruct' H4
+  | ?P ?H0 ?H1 ?H2 ?H3 ?H4 ?H5 => is_ind P; destruct' H0; destruct' H1; destruct' H2; destruct' H3; destruct' H4; destruct' H5
+  | ?P ?H0 ?H1 ?H2 ?H3 ?H4 ?H5 ?H6 => is_ind P; destruct' H0; destruct' H1; destruct' H2; destruct' H3; destruct' H4; destruct' H5; destruct' H6
+  | ?P ?H0 ?H1 ?H2 ?H3 ?H4 ?H5 ?H6 ?H7 => is_ind P; destruct' H0; destruct' H1; destruct' H2; destruct' H3; destruct' H4; destruct' H5; destruct' H6; destruct' H7
+  end || fail "don't know what to destruct".
 
 Theorem nat_ind2: forall (P: nat -> nat -> Prop),
     P 0 0 ->
@@ -318,54 +321,6 @@ Ltac ind_list2_alt x y :=
   | [ |- forall x y, ?H ] => apply (list_ind2_alt (fun x y => H))
   end.
 
-Ltac by_ tactic := tactic; reflexivity.
-Ltac remove_existTs :=
-  repeat lazymatch goal with
-  | H : existT (fun x0 : Set => x0) (js_record ?T) ?a =
-        existT (fun x1 : Set => x1) (list (string * ?T)) ?b |- _ =>
-      unfold js_record in H; apply inj_pair2 in H
-  | H : existT (fun x0 : Set => x0) ?T ?a = existT (fun x1 : Set => x1) ?T ?b |- _ => apply inj_pair2 in H
-  end.
-Ltac clear_obvious :=
-  repeat lazymatch goal with
-  | H : ?T = ?T |- _ => clear H
-  | H : True |- _ => clear H
-  end.
-Ltac inv H := inversion H; remove_existTs; clear_obvious; subst; clear H; try discriminate.
-Ltac if_some tac H := lazymatch H with | None => idtac | @None => idtac | Some ?H => tac H | ?H => idtac H; fail "must be None or Some" end.
-
-Ltac invert_eqs :=
-  repeat lazymatch goal with
-  | H : ?f ?a ?a0 ?a1 ?a2 ?a3 ?a4 ?a5 = ?f ?b ?b0 ?b1 ?b2 ?b3 ?b4 ?b5 |- _ => inv H
-  | H : ?f ?a ?a0 ?a1 ?a2 ?a3 ?a4 = ?f ?b ?b0 ?b1 ?b2 ?b3 ?b4 |- _ => inv H
-  | H : ?f ?a ?a0 ?a1 ?a2 ?a3 = ?f ?b ?b0 ?b1 ?b2 ?b3 |- _ => inv H
-  | H : ?f ?a ?a0 ?a1 ?a2 = ?f ?b ?b0 ?b1 ?b2 |- _ => inv H
-  | H : ?f ?a ?a0 ?a1 = ?f ?b ?b0 ?b1 |- _ => inv H
-  | H : ?f ?a ?a0 = ?f ?b ?b0 |- _ => inv H
-  | H : ?f ?a = ?f ?b |- _ => inv H
-  | H : ?a = nil |- _ => rewrite H in *; clear H
-  end.
-
-Ltac revert_with t :=
-  repeat lazymatch goal with
-  | H : context[t] |- _ => revert H
-  end.
-
-Ltac assert_specialize H :=
-  let tH := type of H in
-  match tH with
-  | ?tHH -> ?tHC =>
-      let HH := fresh "HH" in
-      assert (HH : tHH); [clear H | specialize (H HH); clear HH]
-  | ?tHH <-> ?tHC => apply proj1 in H; assert_specialize H
-  end.
-
-Ltac split_with H :=
-  split; [destruct H as [H _] | destruct H as [_ H]].
-
-Ltac left_right_with H :=
-  destruct H as [H | H]; [left | right].
-
 Lemma list_add_ind : forall {A: Type} (P: list A -> Prop),
     P nil ->
     (forall xs xs', P xs -> (exists x, List.Add x xs xs') -> P xs') ->
@@ -373,258 +328,3 @@ Lemma list_add_ind : forall {A: Type} (P: list A -> Prop),
 Proof.
   intros A P P0 Pn xs; induction xs; [exact P0 | apply (Pn xs); [exact IHxs |]]. exists a. apply List.Add_head.
 Qed.
-
-Ltac rewrite_Forall_Exists_neg A key :=
-  let H := fresh "H" in
-  replace (fun '(key', _) => key <> key') with (fun (x: string * A) => not ((fun '(key', _) => key = key') x)) in *;
-  try (apply functional_extensionality; intros H; destruct H; reflexivity);
-  rewrite List.Forall_Exists_neg in *.
-
-Theorem JsRecordHasKey_dec: forall {A: Set} (key: string) (xs: js_record A),
-    JsRecordHasKey key xs \/ not (JsRecordHasKey key xs).
-Proof.
-  intros; induction xs.
-  - right; intros H; inversion H.
-  - destruct a; destruct (string_dec key s).
-    + left; subst; apply List.Exists_cons_hd; reflexivity.
-    + destruct IHxs; [left | right].
-      * apply List.Exists_cons_tl; exact H.
-      * intros H0; inversion H0; subst.
-        --  contradiction (n eq_refl).
-        --  contradiction (H H2).
-Qed.
-
-Theorem JsRecordHasKey_neg: forall {A: Set} (key: string) (xs: js_record A),
-    not (JsRecordHasKey key xs) <-> List.Forall (fun '(key', _) => key <> key') xs.
-Proof.
-  split; intros; rewrite_Forall_Exists_neg A key; exact H.
-Qed.
-
-Theorem JsRecordHasKey_alt: forall {A: Set} (key: string) (xs: js_record A),
-    JsRecordHasKey key xs <-> not (List.Forall (fun '(key', _) => key <> key') xs).
-Proof.
-  split; intros; rewrite_Forall_Exists_neg A key.
-  - intros H0; contradiction (H0 H).
-  - apply Decidable.not_not; unfold Decidable.decidable; [apply JsRecordHasKey_dec | exact H].
-Qed.
-
-Theorem JsRecordHasKey_neg_Add : forall {A: Set} (kx' : string) (xs': js_record A),
-  not (JsRecordHasKey kx' xs') ->
-  forall (kx: string) (vx: A) (xs: js_record A),
-  List.Add (kx, vx) xs xs' ->
-  kx' <> kx /\ not (JsRecordHasKey kx' xs).
-Proof.
-  intros A kx' xs'; induction xs'; intros; inv H0; rewrite JsRecordHasKey_neg in *; inv H.
-  - split; assumption.
-  - destruct a; subst; rename s into kx0; split.
-    + intros H; subst. rewrite List.Forall_forall in H4; pose (H := List.Add_in H3); pose (H0 := List.in_eq (kx, vx) l); rewrite <- H in H0; specialize (H4 _ H0); simpl in H4; contradiction (H4 eq_refl).
-    + apply List.Forall_cons; [exact H2 |]. rewrite <- JsRecordHasKey_neg; eapply proj2; eapply (IHxs' H4); exact H3.
-Qed.
-
-Corollary JsRecordHasKey_neg_Add0 : forall {A: Set} (kx' : string) (xs': js_record A),
-  not (JsRecordHasKey kx' xs') ->
-  forall (kx: string) (vx: A) (xs: js_record A),
-  List.Add (kx, vx) xs xs' ->
-  not (JsRecordHasKey kx' xs).
-Proof.
-  intros; eapply proj2; eapply JsRecordHasKey_neg_Add; [exact H | exact H0].
-Qed.
-
-Lemma JsRecordNoDup_alt0 : forall {A: Set} (xs': js_record A),
-  JsRecordNoDup xs' ->
-  forall (kx: string) (vx: A) (xs: js_record A),
-  List.Add (kx, vx) xs xs' ->
-  JsRecordNoDup xs.
-Proof.
-  intros A xs'; induction xs'; intros; inv H0; inv H; [exact H2 |]; apply JsRecordNoDup_cons.
-  - apply (IHxs' H2 kx vx); exact H3.
-  - eapply (JsRecordHasKey_neg_Add0 H4); exact H3.
-Qed.
-
-Lemma JsRecordNoDup_alt1 : forall {A: Set} (xs': js_record A),
-  JsRecordNoDup xs' ->
-  forall (kx: string) (vx: A) (xs: js_record A),
-  List.Add (kx, vx) xs xs' ->
-  not (JsRecordHasKey kx xs).
-Proof.
-  intros A xs'; induction xs'; intros; inv H0; inv H; [exact H4 |]; rewrite JsRecordHasKey_neg; apply List.Forall_cons.
-  - intros H; subst; rewrite JsRecordHasKey_neg, List.Forall_forall in H4; pose (H := List.Add_in H3); pose (H0 := List.in_eq (kx0, vx) l); rewrite <- H in H0; specialize (H4 _ H0); simpl in H4; contradiction (H4 eq_refl).
-  - rewrite <- JsRecordHasKey_neg. eapply IHxs'; [exact H2 | exact H3].
-Qed.
-
-Theorem JsRecordNoDup_alt : forall {A: Set} (kx: string) (vx: A) (xs xs': js_record A),
-  JsRecordNoDup xs' ->
-  List.Add (kx, vx) xs xs' ->
-  JsRecordNoDup xs /\ not (JsRecordHasKey kx xs).
-Proof.
-  split; [eapply JsRecordNoDup_alt0 | eapply JsRecordNoDup_alt1]; [exact H | exact H0 | exact H | exact H0].
-Qed.
-
-Theorem JsRecordAdd_HasKey : forall {A: Set} (kx: string) (vx: A) (xs xs': js_record A),
-    JsRecordAdd kx vx xs xs' -> JsRecordHasKey kx xs'.
-Proof.
-  intros. induction H; [apply List.Exists_cons_hd; reflexivity | apply List.Exists_cons_tl; exact IHJsRecordAdd].
-Qed.
-
-Theorem JsRecordAdd_ListAdd : forall {A: Set} (kx: string) (vx: A) (xs xs': js_record A),
-    JsRecordAdd kx vx xs xs' -> List.Add (kx, vx) xs xs'.
-Proof.
-  intros. induction H; constructor. exact IHJsRecordAdd.
-Qed.
-
-Theorem JsRecordAdd_Forall : forall {A: Set} (P: A -> Prop) (kx: string) (vx: A) (xs xs': js_record A),
-    JsRecordAdd kx vx xs xs' -> JsRecordForall P xs' -> P vx /\ JsRecordForall P xs.
-Proof.
-  intros. apply JsRecordAdd_ListAdd in H. unfold JsRecordForall in *. rewrite List.Forall_forall in *. split.
-  - specialize (H0 (kx, vx)). simpl in H0. apply H0. rewrite (List.Add_in H). simpl. left. reflexivity.
-  - intros. specialize (H0 x). destruct x as [kx0 vx0]. simpl in *. apply H0. rewrite (List.Add_in H). simpl. right. exact H1.
-Qed.
-
-Theorem js_record_ind : forall {A: Set} (P: js_record A -> Prop),
-    P nil ->
-    (forall xs xs', P xs -> (exists kx vx, JsRecordAdd kx vx xs xs') -> P xs') ->
-    forall xs, P xs.
-Proof.
-  intros A P P0 Pn xs. induction xs; [exact P0 | apply (Pn xs); [exact IHxs |]]. destruct a as [kx vx]. exists kx. exists vx. apply JsRecordAdd_head.
-Qed.
-
-Theorem js_record_ind2_dumb : forall {A: Set} (P: js_record A -> js_record A -> Prop),
-    P nil nil ->
-    (forall xs xs', P xs nil -> (exists kx vx, JsRecordAdd kx vx xs xs') -> P xs' nil) ->
-    (forall ys ys', P nil ys -> (exists ky vy, JsRecordAdd ky vy ys ys') -> P nil ys') ->
-    (forall xs ys xs' ys', P xs ys -> (exists kx vx, JsRecordAdd kx vx xs xs') -> (exists ky vy, JsRecordAdd ky vy ys ys') -> P xs' ys') ->
-    forall xs ys, P xs ys.
-Proof.
-  intros A P P0 Px Py Pxy xs. induction xs; intros; induction ys; [exact P0 | apply (Py ys); [exact IHys |] | apply (Px xs); [exact (IHxs nil) |] | apply (Pxy xs ys); [exact (IHxs ys) | |] ].
-  - destruct a as [ky vy]. exists ky. exists vy. apply JsRecordAdd_head.
-  - destruct a as [kx vx]. exists kx. exists vx. apply JsRecordAdd_head.
-  - destruct a as [kx vx]. destruct a0 as [ky vy]. exists kx. exists vx. apply JsRecordAdd_head.
-  - destruct a as [kx vx]. destruct a0 as [ky vy]. exists ky. exists vy. apply JsRecordAdd_head.
-Qed.
-
-Ltac ind_js_record2_dumb x y :=
-  revert x y;
-  match goal with
-  | [ |- forall x y, ?H ] => apply (js_record_ind2_dumb (fun x y => H))
-  end.
-
-Theorem JsRecordEqKeys_nil : forall {A: Set}, JsRecordEqKeys (@nil (string * A)) nil.
-Proof.
-  intros A k; split; intros; exact H.
-Qed.
-
-Theorem JsRecordEqKeys_not_cons_nil : forall {A: Set} (x: string * A) (xs: js_record A), ~JsRecordEqKeys (x :: xs)%list nil.
-Proof.
-  intros. intros H. destruct x as [kx vx]. specialize (H kx). assert_specialize H; [apply List.Exists_cons_hd; reflexivity |]. inv H.
-Qed.
-
-Theorem JsRecordEqKeys_not_nil_cons : forall {A: Set} (y: string * A) (ys: js_record A), ~JsRecordEqKeys nil (y :: ys)%list.
-Proof.
-  intros. intros H. destruct y as [ky vy]. specialize (H ky). destruct H as [_ H]. assert_specialize H; [apply List.Exists_cons_hd; reflexivity |]. inv H.
-Qed.
-
-Theorem JsRecordEqKeys_cons : forall {A: Set} (k: string) (vx vy: A) (xs ys: js_record A),
-    JsRecordEqKeys xs ys <-> JsRecordEqKeys ((k, vx) :: xs)%list ((k, vy) :: ys)%list.
-      (* * intros k. split; intros.
-        all: inv H0; [apply List.Exists_cons_hd; reflexivity | apply List.Exists_cons_tl]; apply H; exact H2.
-      * intros H0. contradict H. intros k. split; intros.
-        --  assert (JsRecordHasKey k ((ky, vx) :: xs)%list); [apply List.Exists_cons_tl; exact H |].
-            apply H0 in H1. apply List.Exists_cons in H1. destruct H1.
-            ++  subst. *)
-Admitted.
-
-Theorem JsRecordEqKeys_add : forall {A: Set} (k: string) (vx vy: A) (xs ys xs' ys': js_record A),
-    List.Add (k, vx) xs xs' -> List.Add (k, vy) ys ys' -> (JsRecordEqKeys xs ys <-> JsRecordEqKeys xs' ys').
-      (* * intros k. split; intros.
-        all: inv H0; [apply List.Exists_cons_hd; reflexivity | apply List.Exists_cons_tl]; apply H; exact H2.
-      * intros H0. contradict H. intros k. split; intros.
-        --  assert (JsRecordHasKey k ((ky, vx) :: xs)%list); [apply List.Exists_cons_tl; exact H |].
-            apply H0 in H1. apply List.Exists_cons in H1. destruct H1.
-            ++  subst. *)
-Admitted.
-
-Theorem JsRecordAdd_destruct : forall {A: Set} (kx: string) (vx: A) (xs xs': js_record A),
-    JsRecordAdd kx vx xs xs' <-> (List.Add (kx, vx) xs xs' /\ ~JsRecordHasKey kx xs).
-Admitted.
-
-Theorem JsRecordEqKeys_0 : forall {A: Set} (xs ys: js_record A), JsRecordEqKeys xs ys <-> JsRecordEqKeys0 xs ys.
-Proof.
-  intros; ind_js_record2_dumb xs ys; split; intros.
-  - constructor.
-  - apply JsRecordEqKeys_nil.
-  - destruct xs'; [apply JsRecordEqKeys0_nil | apply JsRecordEqKeys_not_cons_nil in H1; contradiction H1].
-  - destruct xs'; [apply JsRecordEqKeys_nil | inv H1; inv H4].
-  - destruct ys'; [apply JsRecordEqKeys0_nil | apply JsRecordEqKeys_not_nil_cons in H1; contradiction H1].
-  - destruct ys'; [apply JsRecordEqKeys_nil | inv H1; inv H3].
-  - destruct H0 as [kx [vx H0]]; destruct H1 as [ky [vy H1]]. apply JsRecordAdd_destruct in H0. apply JsRecordAdd_destruct in H1. destruct H0. destruct H1. destruct (string_dec kx ky).
-    + subst. clear H3. clear H4. eapply JsRecordEqKeys0_add; [apply H | exact H0 | exact H1]. apply (JsRecordEqKeys_add H0 H1). exact H2.
-    +
-Admitted.
-
-Theorem JsRecordEqKeys_sub_cons : forall {A: Set} (kx ky: string) (vx vy: A) (xs ys: js_record A),
-    JsRecordEqKeys xs ys -> (JsRecordEqKeys ((kx, vx) :: xs)%list ((ky, vy) :: ys)%list <-> kx = ky).
-Admitted.
-
-Theorem JsRecordEqKeys_dec : forall {A: Set} (xs ys: js_record A),
-    JsRecordEqKeys xs ys \/ not (JsRecordEqKeys xs ys).
-Proof.
-  intros. ind_list2 xs ys; intros.
-  - left. apply JsRecordEqKeys_nil.
-  - right. apply JsRecordEqKeys_not_cons_nil.
-  - right. apply JsRecordEqKeys_not_nil_cons.
-  - destruct x as [kx vx]. destruct y as [ky vy]. destruct (string_dec kx ky).
-    + subst. left_right_with H.
-      * apply JsRecordEqKeys_cons. exact H.
-      * intros H0. apply JsRecordEqKeys_cons in H0. contradiction (H H0).
-    + right. intros H0. destruct H.
-      *
-      specialize (H0 kx). assert_specialize H0; [apply List.Exists_cons_hd; reflexivity |].
-      inv H0; [contradiction (n eq_refl) |].
-Admitted.
-
-Theorem js_record_ind2 : forall {A: Set} (P: js_record A -> js_record A -> Prop),
-    P nil nil ->
-    (forall xs xs', P xs nil -> (exists kx vx, JsRecordAdd kx vx xs xs') -> P xs' nil) ->
-    (forall ys ys', P nil ys -> (exists ky vy, JsRecordAdd ky vy ys ys') -> P nil ys') ->
-    (forall xs ys xs' ys', P xs ys -> (JsRecordEqKeys xs ys -> JsRecordEqKeys xs' ys') -> (exists k, (exists vx, JsRecordAdd k vx xs xs') /\ (exists vy, JsRecordAdd k vy ys ys')) -> P xs' ys') ->
-    forall xs ys, P xs ys.
-Admitted.
-
-Ltac ind_js_record2 x y :=
-  revert x y;
-  match goal with
-  | [ |- forall x y, ?H ] => apply (js_record_ind2 (fun x y => H))
-  end.
-
-Theorem js_record_ind3 : forall {A: Set} (P: js_record A -> js_record A -> js_record A -> Prop),
-    P nil nil nil ->
-    (forall xs xs', P xs nil nil -> (exists kx vx, JsRecordAdd kx vx xs xs') -> P xs' nil nil) ->
-    (forall ys ys', P nil ys nil -> (exists ky vy, JsRecordAdd ky vy ys ys') -> P nil ys' nil) ->
-    (forall zs zs', P nil nil zs -> (exists kz vz, JsRecordAdd kz vz zs zs') -> P nil nil zs') ->
-    (forall xs ys xs' ys', P xs ys nil -> (JsRecordEqKeys xs ys -> JsRecordEqKeys xs' ys') -> (exists k, (exists vx, JsRecordAdd k vx xs xs') /\ (exists vy, JsRecordAdd k vy ys ys')) -> P xs' ys' nil) ->
-    (forall xs zs xs' zs', P xs nil zs -> (JsRecordEqKeys xs zs -> JsRecordEqKeys xs' zs') -> (exists k, (exists vx, JsRecordAdd k vx xs xs') /\ (exists vz, JsRecordAdd k vz zs zs')) -> P xs' nil zs') ->
-    (forall ys zs ys' zs', P nil ys zs -> (JsRecordEqKeys ys zs -> JsRecordEqKeys ys' zs') -> (exists k, (exists vy, JsRecordAdd k vy ys ys') /\ (exists vz, JsRecordAdd k vz zs zs')) -> P nil ys' zs') ->
-    (forall xs ys zs xs' ys' zs', P xs ys zs -> (JsRecordEqKeys xs ys -> JsRecordEqKeys xs' ys') -> (JsRecordEqKeys xs zs -> JsRecordEqKeys xs' zs') -> (JsRecordEqKeys ys zs -> JsRecordEqKeys ys' zs') -> (exists k, (exists vx, JsRecordAdd k vx xs xs') /\ (exists vy, JsRecordAdd k vy ys ys') /\ (exists vz, JsRecordAdd k vz zs zs')) -> P xs' ys' zs') ->
-    forall xs ys zs, P xs ys zs.
-Admitted.
-
-Ltac ind_js_record3 x y z :=
-  revert x y z;
-  match goal with
-  | [ |- forall x y z, ?H ] => apply (js_record_ind3 (fun x y z => H))
-  end.
-
-Ltac destruct_var H := is_var H; destruct H.
-
-Ltac destruct' H :=
-  destruct_var H || lazymatch H with
-  | ?P => is_ind P || is_constructor P || is_const P
-  | ?P ?H0 => is_ind P; destruct' H0
-  | ?P ?H0 ?H1 => is_ind P; destruct' H0; destruct' H1
-  | ?P ?H0 ?H1 ?H2 => is_ind P; destruct' H0; destruct' H1; destruct' H2
-  | ?P ?H0 ?H1 ?H2 ?H3 => is_ind P; destruct' H0; destruct' H1; destruct' H2; destruct' H3
-  | ?P ?H0 ?H1 ?H2 ?H3 ?H4 => is_ind P; destruct' H0; destruct' H1; destruct' H2; destruct' H3; destruct' H4
-  | ?P ?H0 ?H1 ?H2 ?H3 ?H4 ?H5 => is_ind P; destruct' H0; destruct' H1; destruct' H2; destruct' H3; destruct' H4; destruct' H5
-  | ?P ?H0 ?H1 ?H2 ?H3 ?H4 ?H5 ?H6 => is_ind P; destruct' H0; destruct' H1; destruct' H2; destruct' H3; destruct' H4; destruct' H5; destruct' H6
-  | ?P ?H0 ?H1 ?H2 ?H3 ?H4 ?H5 ?H6 ?H7 => is_ind P; destruct' H0; destruct' H1; destruct' H2; destruct' H3; destruct' H4; destruct' H5; destruct' H6; destruct' H7
-  end || fail "don't know what to destruct".
