NS/JsRecord.v
@@ -1,0 +1,308 @@
+(* Add LoadPath should not be necessary but it is *)
+Add LoadPath "." as NS.
+Set Implicit Arguments.
+Require Import Coq.Strings.String.
+Require Import Coq.Arith.PeanoNat.
+Require Import Coq.Arith.EqNat.
+Require Import Coq.Bool.Bool.
+Require Import Coq.Logic.FunctionalExtensionality.
+From NS Require Import Misc.
+
+Notation js_record A := (list (string * A)).
+
+Fixpoint js_record_has_key {A: Type} (key: string) (a: js_record A): bool :=
+match a with
+| nil => false
+| cons (x_key, _) xs => String.eqb key x_key || js_record_has_key key xs
+end.
+
+Fixpoint js_record_assoc {A: Type} (key: string) (a: js_record A): option A :=
+match a with
+| nil => None
+| cons (x_key, x) xs => if String.eqb key x_key then Some x else js_record_assoc key xs
+end.
+
+Definition map_js_record {A B: Type} (f: A -> B) (a: js_record A): js_record B :=
+  List.map (fun x => match x with (name, value) => (name, f value) end) a.
+
+Fixpoint js_record_fields_superset {A B: Type} (a: js_record A) (b: js_record B): bool :=
+match b with
+| nil => true
+| cons (b_key, _) bs => js_record_has_key b_key a && js_record_fields_superset a bs
+end.
+
+Definition js_record_fields_eqb {A B: Type} (a: js_record A) (b: js_record B): bool :=
+  js_record_fields_superset a b && js_record_fields_superset b a.
+
+Fixpoint js_record_zip_with {A B C: Type} (f: A -> B -> C) (a: js_record A) (b: js_record B): js_record C :=
+match a with
+| nil => nil
+| cons (x_key, x) xs =>
+    cons_opt (option_map ((fun z => (x_key, z)) << f x) (js_record_assoc x_key b)) (js_record_zip_with f xs b)
+end.
+
+Definition JsRecordForall {A: Type} (P: A -> Prop) : js_record A -> Prop := List.Forall (P << snd).
+
+Definition JsRecordHasKey {A: Type} (key: string): js_record A -> Prop :=
+  List.Exists (fun '(key', _) => key = key').
+
+Definition JsRecordSuperKeys {A: Type} (xs ys: js_record A): Prop :=
+  forall k, JsRecordHasKey k xs -> JsRecordHasKey k ys.
+
+Definition JsRecordEqKeys {A: Type} (xs ys: js_record A): Prop :=
+  forall k, JsRecordHasKey k xs <-> JsRecordHasKey k ys.
+
+Inductive JsRecordEqKeys0 {A: Type}: js_record A -> js_record A -> Prop :=
+| JsRecordEqKeys0_nil : JsRecordEqKeys0 nil nil
+| JsRecordEqKeys0_add : forall (k: string) (vx vy: A) (xs ys xs' ys': js_record A), JsRecordEqKeys0 xs ys -> List.Add (k, vx) xs xs' -> List.Add (k, vy) ys ys' -> JsRecordEqKeys0 xs' ys'
+.
+
+Inductive JsRecordAdd {A: Type} (kx: string) (vx: A) : js_record A -> js_record A -> Prop :=
+| JsRecordAdd_head : forall (xs: js_record A), JsRecordAdd kx vx xs ((kx, vx) :: xs)%list
+| JsRecordAdd_cons : forall (kx0: string) (vx0: A) (xs xs': js_record A), kx0 <> kx -> JsRecordAdd kx vx xs xs' -> JsRecordAdd kx vx ((kx0, vx0) :: xs)%list ((kx0, vx0) :: xs')%list
+.
+
+Inductive JsRecordNoDup {A: Type} : js_record A -> Prop :=
+| JsRecordNoDup_nil : JsRecordNoDup nil
+| JsRecordNoDup_cons : forall kx vx xs, JsRecordNoDup xs -> not (JsRecordHasKey kx xs) -> JsRecordNoDup ((kx, vx) :: xs)%list
+.
+
+Ltac rewrite_Forall_Exists_neg A key :=
+  let H := fresh "H" in
+  replace (fun '(key', _) => key <> key') with (fun (x: string * A) => not ((fun '(key', _) => key = key') x)) in *;
+  try (apply functional_extensionality; intros H; destruct H; reflexivity);
+  rewrite List.Forall_Exists_neg in *.
+
+Theorem JsRecordHasKey_dec: forall {A: Type} (key: string) (xs: js_record A),
+    JsRecordHasKey key xs \/ not (JsRecordHasKey key xs).
+Proof.
+  intros; induction xs.
+  - right; intros H; inversion H.
+  - destruct a; destruct (string_dec key s).
+    + left; subst; apply List.Exists_cons_hd; reflexivity.
+    + destruct IHxs; [left | right].
+      * apply List.Exists_cons_tl; exact H.
+      * intros H0; inversion H0; subst.
+        --  contradiction (n eq_refl).
+        --  contradiction (H H2).
+Qed.
+
+Theorem JsRecordHasKey_neg: forall {A: Type} (key: string) (xs: js_record A),
+    not (JsRecordHasKey key xs) <-> List.Forall (fun '(key', _) => key <> key') xs.
+Proof.
+  split; intros; rewrite_Forall_Exists_neg A key; exact H.
+Qed.
+
+Theorem JsRecordHasKey_alt: forall {A: Type} (key: string) (xs: js_record A),
+    JsRecordHasKey key xs <-> not (List.Forall (fun '(key', _) => key <> key') xs).
+Proof.
+  split; intros; rewrite_Forall_Exists_neg A key.
+  - intros H0; contradiction (H0 H).
+  - apply Decidable.not_not; unfold Decidable.decidable; [apply JsRecordHasKey_dec | exact H].
+Qed.
+
+Theorem JsRecordHasKey_neg_Add : forall {A: Type} (kx' : string) (xs': js_record A),
+  not (JsRecordHasKey kx' xs') ->
+  forall (kx: string) (vx: A) (xs: js_record A),
+  List.Add (kx, vx) xs xs' ->
+  kx' <> kx /\ not (JsRecordHasKey kx' xs).
+Proof.
+  intros A kx' xs'; induction xs'; intros; inv H0; rewrite JsRecordHasKey_neg in *; inv H.
+  - split; assumption.
+  - destruct a; subst; rename s into kx0; split.
+    + intros H; subst. rewrite List.Forall_forall in H4; pose (H := List.Add_in H3); pose (H0 := List.in_eq (kx, vx) l); rewrite <- H in H0; specialize (H4 _ H0); simpl in H4; contradiction (H4 eq_refl).
+    + apply List.Forall_cons; [exact H2 |]. rewrite <- JsRecordHasKey_neg; eapply proj2; eapply (IHxs' H4); exact H3.
+Qed.
+
+Corollary JsRecordHasKey_neg_Add0 : forall {A: Type} (kx' : string) (xs': js_record A),
+  not (JsRecordHasKey kx' xs') ->
+  forall (kx: string) (vx: A) (xs: js_record A),
+  List.Add (kx, vx) xs xs' ->
+  not (JsRecordHasKey kx' xs).
+Proof.
+  intros; eapply proj2; eapply JsRecordHasKey_neg_Add; [exact H | exact H0].
+Qed.
+
+Lemma JsRecordNoDup_alt0 : forall {A: Type} (xs': js_record A),
+  JsRecordNoDup xs' ->
+  forall (kx: string) (vx: A) (xs: js_record A),
+  List.Add (kx, vx) xs xs' ->
+  JsRecordNoDup xs.
+Proof.
+  intros A xs'; induction xs'; intros; inv H0; inv H; [exact H2 |]; apply JsRecordNoDup_cons.
+  - apply (IHxs' H2 kx vx); exact H3.
+  - eapply (JsRecordHasKey_neg_Add0 H4); exact H3.
+Qed.
+
+Lemma JsRecordNoDup_alt1 : forall {A: Type} (xs': js_record A),
+  JsRecordNoDup xs' ->
+  forall (kx: string) (vx: A) (xs: js_record A),
+  List.Add (kx, vx) xs xs' ->
+  not (JsRecordHasKey kx xs).
+Proof.
+  intros A xs'; induction xs'; intros; inv H0; inv H; [exact H4 |]; rewrite JsRecordHasKey_neg; apply List.Forall_cons.
+  - intros H; subst; rewrite JsRecordHasKey_neg, List.Forall_forall in H4; pose (H := List.Add_in H3); pose (H0 := List.in_eq (kx0, vx) l); rewrite <- H in H0; specialize (H4 _ H0); simpl in H4; contradiction (H4 eq_refl).
+  - rewrite <- JsRecordHasKey_neg. eapply IHxs'; [exact H2 | exact H3].
+Qed.
+
+Theorem JsRecordNoDup_alt : forall {A: Type} (kx: string) (vx: A) (xs xs': js_record A),
+  JsRecordNoDup xs' ->
+  List.Add (kx, vx) xs xs' ->
+  JsRecordNoDup xs /\ not (JsRecordHasKey kx xs).
+Proof.
+  split; [eapply JsRecordNoDup_alt0 | eapply JsRecordNoDup_alt1]; [exact H | exact H0 | exact H | exact H0].
+Qed.
+
+Theorem JsRecordAdd_HasKey : forall {A: Type} (kx: string) (vx: A) (xs xs': js_record A),
+    JsRecordAdd kx vx xs xs' -> JsRecordHasKey kx xs'.
+Proof.
+  intros. induction H; [apply List.Exists_cons_hd; reflexivity | apply List.Exists_cons_tl; exact IHJsRecordAdd].
+Qed.
+
+Theorem JsRecordAdd_ListAdd : forall {A: Type} (kx: string) (vx: A) (xs xs': js_record A),
+    JsRecordAdd kx vx xs xs' -> List.Add (kx, vx) xs xs'.
+Proof.
+  intros. induction H; constructor. exact IHJsRecordAdd.
+Qed.
+
+Theorem JsRecordAdd_Forall : forall {A: Type} (P: A -> Prop) (kx: string) (vx: A) (xs xs': js_record A),
+    JsRecordAdd kx vx xs xs' -> JsRecordForall P xs' -> P vx /\ JsRecordForall P xs.
+Proof.
+  intros. apply JsRecordAdd_ListAdd in H. unfold JsRecordForall in *. rewrite List.Forall_forall in *. split.
+  - specialize (H0 (kx, vx)). simpl in H0. apply H0. rewrite (List.Add_in H). simpl. left. reflexivity.
+  - intros. specialize (H0 x). destruct x as [kx0 vx0]. simpl in *. apply H0. rewrite (List.Add_in H). simpl. right. exact H1.
+Qed.
+
+Theorem js_record_ind : forall {A: Type} (P: js_record A -> Prop),
+    P nil ->
+    (forall xs xs', P xs -> (exists kx vx, JsRecordAdd kx vx xs xs') -> P xs') ->
+    forall xs, P xs.
+Proof.
+  intros A P P0 Pn xs. induction xs; [exact P0 | apply (Pn xs); [exact IHxs |]]. destruct a as [kx vx]. exists kx. exists vx. apply JsRecordAdd_head.
+Qed.
+
+Theorem js_record_ind2_dumb : forall {A: Type} (P: js_record A -> js_record A -> Prop),
+    P nil nil ->
+    (forall xs xs', P xs nil -> (exists kx vx, JsRecordAdd kx vx xs xs') -> P xs' nil) ->
+    (forall ys ys', P nil ys -> (exists ky vy, JsRecordAdd ky vy ys ys') -> P nil ys') ->
+    (forall xs ys xs' ys', P xs ys -> (exists kx vx, JsRecordAdd kx vx xs xs') -> (exists ky vy, JsRecordAdd ky vy ys ys') -> P xs' ys') ->
+    forall xs ys, P xs ys.
+Proof.
+  intros A P P0 Px Py Pxy xs. induction xs; intros; induction ys; [exact P0 | apply (Py ys); [exact IHys |] | apply (Px xs); [exact (IHxs nil) |] | apply (Pxy xs ys); [exact (IHxs ys) | |] ].
+  - destruct a as [ky vy]. exists ky. exists vy. apply JsRecordAdd_head.
+  - destruct a as [kx vx]. exists kx. exists vx. apply JsRecordAdd_head.
+  - destruct a as [kx vx]. destruct a0 as [ky vy]. exists kx. exists vx. apply JsRecordAdd_head.
+  - destruct a as [kx vx]. destruct a0 as [ky vy]. exists ky. exists vy. apply JsRecordAdd_head.
+Qed.
+
+Ltac ind_js_record2_dumb x y :=
+  revert x y;
+  match goal with
+  | [ |- forall x y, ?H ] => apply (js_record_ind2_dumb (fun x y => H))
+  end.
+
+Theorem JsRecordEqKeys_nil : forall {A: Type}, JsRecordEqKeys (@nil (string * A)) nil.
+Proof.
+  intros A k; split; intros; exact H.
+Qed.
+
+Theorem JsRecordEqKeys_not_cons_nil : forall {A: Type} (x: string * A) (xs: js_record A), ~JsRecordEqKeys (x :: xs)%list nil.
+Proof.
+  intros. intros H. destruct x as [kx vx]. specialize (H kx). assert_specialize H; [apply List.Exists_cons_hd; reflexivity |]. inv H.
+Qed.
+
+Theorem JsRecordEqKeys_not_nil_cons : forall {A: Type} (y: string * A) (ys: js_record A), ~JsRecordEqKeys nil (y :: ys)%list.
+Proof.
+  intros. intros H. destruct y as [ky vy]. specialize (H ky). destruct H as [_ H]. assert_specialize H; [apply List.Exists_cons_hd; reflexivity |]. inv H.
+Qed.
+
+Theorem JsRecordEqKeys_cons : forall {A: Type} (k: string) (vx vy: A) (xs ys: js_record A),
+    JsRecordEqKeys xs ys <-> JsRecordEqKeys ((k, vx) :: xs)%list ((k, vy) :: ys)%list.
+      (* * intros k. split; intros.
+        all: inv H0; [apply List.Exists_cons_hd; reflexivity | apply List.Exists_cons_tl]; apply H; exact H2.
+      * intros H0. contradict H. intros k. split; intros.
+        --  assert (JsRecordHasKey k ((ky, vx) :: xs)%list); [apply List.Exists_cons_tl; exact H |].
+            apply H0 in H1. apply List.Exists_cons in H1. destruct H1.
+            ++  subst. *)
+Admitted.
+
+Theorem JsRecordEqKeys_add : forall {A: Type} (k: string) (vx vy: A) (xs ys xs' ys': js_record A),
+    List.Add (k, vx) xs xs' -> List.Add (k, vy) ys ys' -> (JsRecordEqKeys xs ys <-> JsRecordEqKeys xs' ys').
+      (* * intros k. split; intros.
+        all: inv H0; [apply List.Exists_cons_hd; reflexivity | apply List.Exists_cons_tl]; apply H; exact H2.
+      * intros H0. contradict H. intros k. split; intros.
+        --  assert (JsRecordHasKey k ((ky, vx) :: xs)%list); [apply List.Exists_cons_tl; exact H |].
+            apply H0 in H1. apply List.Exists_cons in H1. destruct H1.
+            ++  subst. *)
+Admitted.
+
+Theorem JsRecordAdd_destruct : forall {A: Type} (kx: string) (vx: A) (xs xs': js_record A),
+    JsRecordAdd kx vx xs xs' <-> (List.Add (kx, vx) xs xs' /\ ~JsRecordHasKey kx xs).
+Admitted.
+
+Theorem JsRecordEqKeys_0 : forall {A: Type} (xs ys: js_record A), JsRecordEqKeys xs ys <-> JsRecordEqKeys0 xs ys.
+Proof.
+  intros; ind_js_record2_dumb xs ys; split; intros.
+  - constructor.
+  - apply JsRecordEqKeys_nil.
+  - destruct xs'; [apply JsRecordEqKeys0_nil | apply JsRecordEqKeys_not_cons_nil in H1; contradiction H1].
+  - destruct xs'; [apply JsRecordEqKeys_nil | inv H1; inv H4].
+  - destruct ys'; [apply JsRecordEqKeys0_nil | apply JsRecordEqKeys_not_nil_cons in H1; contradiction H1].
+  - destruct ys'; [apply JsRecordEqKeys_nil | inv H1; inv H3].
+  - destruct H0 as [kx [vx H0]]; destruct H1 as [ky [vy H1]]. apply JsRecordAdd_destruct in H0. apply JsRecordAdd_destruct in H1. destruct H0. destruct H1. destruct (string_dec kx ky).
+    + subst. clear H3. clear H4. eapply JsRecordEqKeys0_add; [apply H | exact H0 | exact H1]. apply (JsRecordEqKeys_add H0 H1). exact H2.
+    +
+Admitted.
+
+Theorem JsRecordEqKeys_sub_cons : forall {A: Type} (kx ky: string) (vx vy: A) (xs ys: js_record A),
+    JsRecordEqKeys xs ys -> (JsRecordEqKeys ((kx, vx) :: xs)%list ((ky, vy) :: ys)%list <-> kx = ky).
+Admitted.
+
+Theorem JsRecordEqKeys_dec : forall {A: Type} (xs ys: js_record A),
+    JsRecordEqKeys xs ys \/ not (JsRecordEqKeys xs ys).
+Proof.
+  intros. ind_list2 xs ys; intros.
+  - left. apply JsRecordEqKeys_nil.
+  - right. apply JsRecordEqKeys_not_cons_nil.
+  - right. apply JsRecordEqKeys_not_nil_cons.
+  - destruct x as [kx vx]. destruct y as [ky vy]. destruct (string_dec kx ky).
+    + subst. left_right_with H.
+      * apply JsRecordEqKeys_cons. exact H.
+      * intros H0. apply JsRecordEqKeys_cons in H0. contradiction (H H0).
+    + right. intros H0. destruct H.
+      *
+      specialize (H0 kx). assert_specialize H0; [apply List.Exists_cons_hd; reflexivity |].
+      inv H0; [contradiction (n eq_refl) |].
+Admitted.
+
+Theorem js_record_ind2 : forall {A: Type} (P: js_record A -> js_record A -> Prop),
+    P nil nil ->
+    (forall xs xs', P xs nil -> (exists kx vx, JsRecordAdd kx vx xs xs') -> P xs' nil) ->
+    (forall ys ys', P nil ys -> (exists ky vy, JsRecordAdd ky vy ys ys') -> P nil ys') ->
+    (forall xs ys xs' ys', P xs ys -> (JsRecordEqKeys xs ys -> JsRecordEqKeys xs' ys') -> (exists k, (exists vx, JsRecordAdd k vx xs xs') /\ (exists vy, JsRecordAdd k vy ys ys')) -> P xs' ys') ->
+    forall xs ys, P xs ys.
+Admitted.
+
+Ltac ind_js_record2 x y :=
+  revert x y;
+  match goal with
+  | [ |- forall x y, ?H ] => apply (js_record_ind2 (fun x y => H))
+  end.
+
+Theorem js_record_ind3 : forall {A: Type} (P: js_record A -> js_record A -> js_record A -> Prop),
+    P nil nil nil ->
+    (forall xs xs', P xs nil nil -> (exists kx vx, JsRecordAdd kx vx xs xs') -> P xs' nil nil) ->
+    (forall ys ys', P nil ys nil -> (exists ky vy, JsRecordAdd ky vy ys ys') -> P nil ys' nil) ->
+    (forall zs zs', P nil nil zs -> (exists kz vz, JsRecordAdd kz vz zs zs') -> P nil nil zs') ->
+    (forall xs ys xs' ys', P xs ys nil -> (JsRecordEqKeys xs ys -> JsRecordEqKeys xs' ys') -> (exists k, (exists vx, JsRecordAdd k vx xs xs') /\ (exists vy, JsRecordAdd k vy ys ys')) -> P xs' ys' nil) ->
+    (forall xs zs xs' zs', P xs nil zs -> (JsRecordEqKeys xs zs -> JsRecordEqKeys xs' zs') -> (exists k, (exists vx, JsRecordAdd k vx xs xs') /\ (exists vz, JsRecordAdd k vz zs zs')) -> P xs' nil zs') ->
+    (forall ys zs ys' zs', P nil ys zs -> (JsRecordEqKeys ys zs -> JsRecordEqKeys ys' zs') -> (exists k, (exists vy, JsRecordAdd k vy ys ys') /\ (exists vz, JsRecordAdd k vz zs zs')) -> P nil ys' zs') ->
+    (forall xs ys zs xs' ys' zs', P xs ys zs -> (JsRecordEqKeys xs ys -> JsRecordEqKeys xs' ys') -> (JsRecordEqKeys xs zs -> JsRecordEqKeys xs' zs') -> (JsRecordEqKeys ys zs -> JsRecordEqKeys ys' zs') -> (exists k, (exists vx, JsRecordAdd k vx xs xs') /\ (exists vy, JsRecordAdd k vy ys ys') /\ (exists vz, JsRecordAdd k vz zs zs')) -> P xs' ys' zs') ->
+    forall xs ys zs, P xs ys zs.
+Admitted.
+
+Ltac ind_js_record3 x y z :=
+  revert x y z;
+  match goal with
+  | [ |- forall x y z, ?H ] => apply (js_record_ind3 (fun x y z => H))
+  end.
